check_axioms.sh
@@ -1,0 +1,2 @@
+#! /bin/sh
+grep -n -e 'Axiom' $(find . -name '*.v' -type f)
